Got full List example to verify

Test/dafny0/List.dfy
@@ -14,18 +14,25 @@ trait List {
   method Get(i: int) returns (res: int)
     requires Valid()
     requires 0 <= i < Length()
+    decreases Repr
     ensures res == values[i]
   
   method Set(i: int, element: int)
     requires Valid()
     requires 0 <= i < Length()
+    decreases Repr
     modifies Repr
+    ensures Valid()
     ensures values == old(values[..i]) + [element] + old(values[i + 1..])
-  
+    ensures fresh(Repr - old(Repr))
+    
   method Add(element: int)
     requires Valid()
+    decreases Repr
     modifies Repr
+    ensures Valid()
     ensures values == old(values) + [element]
+    ensures fresh(Repr - old(Repr))
 }
 
 class ArrayList extends List {
@@ -33,9 +40,15 @@ class ArrayList extends List {
   var data: array<int>
   var length: int
 
-  constructor() {
+  constructor() 
+    ensures Valid()
+    ensures values == []
+  {
     data := new int[10];
     length := 0;
+
+    values := [];
+    Repr := {this, data};
   }
 
   predicate Valid()
@@ -59,6 +72,7 @@ class ArrayList extends List {
   method Get(i: int) returns (res: int)
     requires Valid()
     requires 0 <= i < Length()
+    decreases Repr
     ensures res == values[i]
   {
     res := data[i];
@@ -67,19 +81,24 @@ class ArrayList extends List {
   method Set(i: int, element: int)
     requires Valid()
     requires 0 <= i < Length()
+    decreases Repr
     modifies Repr
     ensures Valid()
+    ensures fresh(Repr - old(Repr))
     ensures values == old(values[..i]) + [element] + old(values[i + 1..])
   {
     data[i] := element;
-    
+
     values := values[..i] + [element] + values[i + 1..];
   }
 
   method Add(element: int)
     requires Valid()
+    decreases Repr
     modifies Repr
+    ensures Valid()
     ensures values == old(values) + [element]
+    ensures fresh(Repr - old(Repr))
   {
     if length == data.Length {
       Grow();
@@ -92,9 +111,12 @@ class ArrayList extends List {
 
   method Grow() 
     requires Valid()
-    modifies this`data, data
+    modifies Repr
     ensures length < data.Length
     ensures fresh(data)
+    ensures unchanged(`length)
+    ensures values == old(values)
+    ensures Valid()
   {
     var oldSize := data.Length;
     var newData := new int[2 * data.Length];
@@ -102,5 +124,182 @@ class ArrayList extends List {
       newData[i] := data[i];
     }
     data := newData;
+    
+    Repr := {this, data};
+  }
+}
+
+trait {:extern} ExternalList {
+
+  predicate Valid()
+    reads this, Repr
+    ensures Valid() ==> this in Repr
+  ghost var Repr: set<object>
+
+  function method Length(): int 
+    requires Valid()
+    reads Repr
+    ensures Valid()
+  
+  method Get(i: int) returns (res: int)
+    requires Valid()
+    decreases Repr
+  
+  method Set(i: int, element: int)
+    requires Valid()
+    modifies Repr
+    decreases Repr
+    ensures Valid()
+    ensures fresh(Repr - old(Repr))
+  
+  method Add(element: int)
+    requires Valid()
+    modifies Repr
+    decreases Repr
+    ensures Valid()
+    ensures fresh(Repr - old(Repr))
+}
+
+class AsExternalList extends ExternalList {
+
+  var wrapped: List
+
+  constructor(wrapped: List) 
+    requires wrapped.Valid()
+    ensures Valid()
+  {
+    this.wrapped := wrapped;
+    this.Repr := {this} + wrapped.Repr;
+  }
+
+  predicate Valid()
+    reads this, Repr
+    ensures Valid() ==> this in Repr 
+  {
+    && wrapped in Repr
+    && Repr == {this} + wrapped.Repr
+    && wrapped in wrapped.Repr
+    && this !in wrapped.Repr
+    && wrapped.Repr <= Repr
+    && wrapped.Valid()
+  }
+
+  function method Length(): int 
+    requires Valid()
+    reads Repr
+  {
+    wrapped.Length()
+  }
+  
+  method Get(i: int) returns (res: int)
+    requires Valid()
+    decreases Repr
+  {
+    expect 0 <= i < Length();
+    res := wrapped.Get(i);
+  }
+  
+  method Set(i: int, element: int)
+    requires Valid()
+    modifies Repr
+    decreases Repr
+    ensures Valid()
+    ensures fresh(Repr - old(Repr))
+  {
+    expect 0 <= i < Length();
+    wrapped.Set(i, element);
+    Repr := {this} + wrapped.Repr;
+  }
+  
+  method Add(element: int)
+    requires Valid()
+    modifies Repr
+    decreases Repr
+    ensures Valid()
+    ensures fresh(Repr - old(Repr))
+  {
+    wrapped.Add(element);
+    Repr := {this} + wrapped.Repr;
+  }
+}
+
+class AsList extends List {
+
+  var wrapped: ExternalList
+
+  constructor(wrapped: ExternalList) 
+    requires wrapped.Valid()
+    ensures Valid()
+  {
+    this.wrapped := wrapped;
+    this.Repr := {this} + wrapped.Repr;
+  }
+
+  predicate Valid()
+    reads this, Repr
+    ensures Valid() ==> this in Repr 
+  {
+    && wrapped in Repr
+    && Repr == {this} + wrapped.Repr
+    && wrapped in wrapped.Repr
+    && this !in wrapped.Repr
+    && wrapped.Repr <= Repr
+    && wrapped.Valid()
+  }
+
+  function method Length(): int
+    requires Valid()
+    reads this, Repr
+    ensures Length() == |values|
+  {
+    assume {:axiom} wrapped.Length() == |values|;
+    wrapped.Length()
+  }
+  
+  method Get(i: int) returns (res: int)
+    requires Valid()
+    requires 0 <= i < Length()
+    decreases Repr
+    ensures res == values[i]
+  {
+    res := wrapped.Get(i);
+    assume {:axiom} res == values[i];
+  }
+  
+  method Set(i: int, element: int)
+    requires Valid()
+    requires 0 <= i < Length()
+    decreases Repr
+    modifies Repr
+    ensures Valid()
+    ensures values == old(values[..i]) + [element] + old(values[i + 1..])
+    ensures fresh(Repr - old(Repr))
+  {
+    wrapped.Set(i, element);
+
+    // Presumably cheap sanity check
+    var elementAfter := wrapped.Get(i);
+    expect elementAfter == element;
+
+    values := values[..i] + [element] + values[i + 1..];
+    Repr := {this} + wrapped.Repr;
+  }
+
+  method Add(element: int)
+    requires Valid()
+    decreases Repr
+    modifies Repr
+    ensures Valid()
+    ensures values == old(values) + [element]
+    ensures fresh(Repr - old(Repr))
+  {
+    var lengthBefore := Length();
+
+    wrapped.Add(element);
+
+    values := values + [element];
+    Repr := {this} + wrapped.Repr;
+
+    expect Length() == lengthBefore + 1;
   }
 }
